bedrock2/src/bedrock2/ZnWords.v
@@ -20,6 +20,7 @@ Lemma computable_lt{lo v: Z}(H: Z.ltb lo v = true): lo < v.
 Proof. apply Z.ltb_lt. assumption. Qed.
 
 Ltac cleanup_for_ZModArith :=
+  subst; (* <-- substituting `@eq word _ _` might create opportunities for wordOps_to_ZModArith_step *)
   repeat match goal with
          | a := _ |- _ => subst a
          | H: ?T |- _ => tryif is_lia T then fail else clear H
